powerpc/Conventions1.v
@@ -296,30 +296,28 @@ Opaque list_nth_z.
   destruct (list_nth_z int_param_regs ir) as [r|] eqn:E; destruct H.
   subst. left. eapply list_nth_z_in; eauto.
   eapply IHtyl; eauto.
-  subst. split. lia. apply Z.divide_1_l.
+  subst. split. lia. auto with divide.
   eapply Y; eauto. lia.
 - (* float *)
   assert (ofs <= align ofs 2) by (apply align_le; lia).
   destruct (list_nth_z float_param_regs fr) as [r|] eqn:E; destruct H.
   subst. right. eapply list_nth_z_in; eauto.
   eapply IHtyl; eauto.
-  subst. split. lia. apply Z.divide_1_l.
+  subst. split. lia. auto with divide.
   eapply Y; eauto. lia.
 - (* long *)
   assert (ofs <= align ofs 2) by (apply align_le; lia).
   set (ir' := align ir 2) in *.
-  destruct (list_nth_z int_param_regs ir') as [r1|] eqn:E1.
-  destruct (list_nth_z int_param_regs (ir' + 1)) as [r2|] eqn:E2.
-  destruct H. subst; split; left; eapply list_nth_z_in; eauto.
-  eapply IHtyl; eauto.
-  destruct H.
-  subst. destruct Archi.ptr64; [split|split;split]; try lia.
-  apply align_divides; lia. apply Z.divide_1_l. apply Z.divide_1_l.
-  eapply Y; eauto. lia.
-  destruct H.
-  subst. destruct Archi.ptr64; [split|split;split]; try lia.
-  apply align_divides; lia. apply Z.divide_1_l. apply Z.divide_1_l.
-  eapply Y; eauto. lia.
+  destruct (list_nth_z int_param_regs ir') as [r1|] eqn:E1;
+  [ destruct (list_nth_z int_param_regs (ir' + 1)) as [r2|] eqn:E2 | ].
+  + destruct H. subst; split; left; eapply list_nth_z_in; eauto.
+    eapply IHtyl; eauto.
+  + destruct H.
+    subst. destruct Archi.ptr64; [split|split;split]; try lia; auto with divide.
+    eapply Y; eauto. lia.
+  + destruct H.
+    subst. destruct Archi.ptr64; [split|split;split]; try lia; auto with divide.
+    eapply Y; eauto. lia.
 - (* single *)
   assert (ofs <= align ofs 1) by (apply align_le; lia).
   assert (ofs <= align ofs 2) by (apply align_le; lia).
@@ -327,20 +325,20 @@ Opaque list_nth_z.
   subst. right. eapply list_nth_z_in; eauto.
   eapply IHtyl; eauto.
   subst. split. destruct Archi.single_passed_as_single; simpl; lia.
-  destruct Archi.single_passed_as_single; simpl; apply Z.divide_1_l.
+  destruct Archi.single_passed_as_single; simpl; auto with divide.
   eapply Y; eauto. destruct Archi.single_passed_as_single; simpl; lia.
 - (* any32 *)
   destruct (list_nth_z int_param_regs ir) as [r|] eqn:E; destruct H.
   subst. left. eapply list_nth_z_in; eauto.
   eapply IHtyl; eauto.
-  subst. split. lia. apply Z.divide_1_l.
+  subst. split. lia. auto with divide.
   eapply Y; eauto. lia.
 - (* float *)
   assert (ofs <= align ofs 2) by (apply align_le; lia).
   destruct (list_nth_z float_param_regs fr) as [r|] eqn:E; destruct H.
   subst. right. eapply list_nth_z_in; eauto.
   eapply IHtyl; eauto.
-  subst. split. lia. apply Z.divide_1_l.
+  subst. split. lia. auto with divide.
   eapply Y; eauto. lia.
 Qed.
 
